Prove Day 1 wrt slower impl

Aoc2025/Day01.lean
@@ -1,86 +1,40 @@
+import Std.Tactic.Do
+
 namespace Day01
 
-abbrev dialSize : Int := 100
-structure Dial where
-  toInt : Int
-  isNormalised : toInt = toInt % dialSize
-
-def dialInit : Dial := ⟨50, by grind⟩
-
-theorem Dial.toInt_nonneg (d : Dial) : 0 <= d.toInt := by
-  rw [d.isNormalised]; grind
+abbrev dialSize : Nat := 100
+abbrev Dial := Fin dialSize
+def dialInit : Dial := 50
 
 /-- Note: DialState α over a monoid ⟨α, ×⟩ has the monoidal
   structure ((×) <$> · <*> ·), which we will define
   homomorphisms into. -/
 abbrev DialState α := StateM Dial α
 
+def stepDial0 (command : Int) (dial : Dial) : Dial :=
+  ⟨((dial + command) % dialSize).toNat, (by grind)⟩
+
 -- Rotate the dial by the given command.
 def stepDial (command : Int) : DialState Unit := do
-  let dial <- get
-  set $ Dial.mk ((dial.toInt + command) % dialSize) (by grind)
-
-/-- stepDial is a monoid homomorphism (ℤ, +) → DialState Unit. -/
-theorem stepDial_hom (c0 c1 : Int)
-  : stepDial (c0 + c1) = stepDial c0 *> stepDial c1 := by
-  intros; ext
-  simp [stepDial]
-  grind
-
-@[simp]
-theorem stepDial_zero : stepDial 0 = pure ⟨⟩ := by
-  ext d; simp [stepDial]; congr
-  rw [← d.isNormalised]
+  modify (stepDial0 command)
 
 -- Rotate the dial at once, only counting 0 at the end.
 def stepAtomic (command : Int) : DialState Nat := do
   stepDial command
   let dial' <- get
-  return if dial'.toInt = 0 then 1 else 0
+  return if dial' = 0 then 1 else 0
 
 -- Rotate the dial one step at a time, counting every 0.
 def stepIncrementalSlow (command : Int) : DialState Nat :=
   List.sum <$> (List.replicate command.natAbs command.sign).mapM stepAtomic
 
-theorem Int.add_same_sign_eq (c0 c1 : Int)
-  : c0.sign = c1.sign →
-    (c0 + c1).sign = c1.sign := by
-  intro
-  if _ : c1 = 0
-  then grind [Int.eq_zero_of_sign_eq_zero]
-  else if _ : c1 > 0
-  then grind [Int.sign_eq_one_iff_pos]
-  else grind [Int.sign_eq_neg_one_iff_neg]
-
-theorem Int.natAbs_add_of_same_sign (c0 c1 : Int)
-  : c0.sign = c1.sign →
-    (c0 + c1).natAbs = c0.natAbs + c1.natAbs := by
-  intro
-  if _ : c1 = 0 then grind
-  else if _ : c1 > 0
-  then grind [Int.sign_eq_one_iff_pos, Int.natAbs_add_of_nonneg]
-  else grind [Int.sign_eq_neg_one_iff_neg, Int.natAbs_add_of_nonpos]
-
-/- stepIncrementalSlow is a monoid homomorphism
- from the fixed-signed integers to DialState Nat. -/
-theorem stepIncrementalSlow_hom (c0 c1 : Int)
-  : c0.sign = c1.sign →
-    stepIncrementalSlow (c0 + c1)
-    = ((· + ·) <$> stepIncrementalSlow c0 <*> stepIncrementalSlow c1) := by
-  intros hsign; apply StateT.ext; intro dial0
-  simp [stepIncrementalSlow]
-  rw [Int.natAbs_add_of_same_sign _ _ hsign,
-       ← List.replicate_append_replicate, List.mapM_append,
-       Int.add_same_sign_eq _ _ hsign, hsign]
-  simp
-
-/- we could probably show that this is also a monoid homomorphism -/
+-- This is proven to be equivalent to stepIncrementalSlow above.
 def stepIncremental (command : Int) : DialState Nat := do
   let dial <- get
   stepDial command
-  let rawDial' := dial.toInt + command
-  let mut fullRotations := (rawDial'.natAbs / dialSize).natAbs
-  if rawDial' <= 0 ∧ dial.toInt != 0 then
+  let rawDial' := dial + command
+  let mut fullRotations := rawDial'.natAbs / dialSize
+  if rawDial' ≤ 0 ∧ dial ≠ 0 then
     fullRotations := fullRotations + 1
   return fullRotations
 
@@ -122,3 +76,212 @@ def main : IO Unit := do
   IO.println s!"Part 1: {part1 commands}"
   IO.println s!"Part 2: {part2 commands}"
   return ()
+
+-- Proofs
+namespace Day01
+open Day01
+
+theorem Dial.toInt_nonneg (d : Dial) : 0 <= ↑d := by grind
+
+@[grind]
+theorem Dial.lt_dialSize (dial : Dial) : dial < (dialSize : Int) := by
+  norm_cast ; grind
+
+/-- stepDial is a monoid homomorphism (ℤ, +) → DialState Unit. -/
+theorem stepDial_hom (c0 c1 : Int)
+  : stepDial (c0 + c1) = stepDial c0 *> stepDial c1 := by
+  intros; ext
+  simp [stepDial, stepDial0]
+  grind
+
+@[simp]
+theorem stepDial_zero : stepDial 0 = pure () := by
+  ext d; simp [stepDial, stepDial0]; congr
+  suffices ↑↑d % 100 = ↑↑d by grind
+  grind
+
+theorem Int.add_same_sign_eq (c0 c1 : Int)
+  : c0.sign = c1.sign →
+    (c0 + c1).sign = c1.sign := by
+  intro
+  if _ : c1 = 0
+  then grind [Int.eq_zero_of_sign_eq_zero]
+  else if _ : c1 > 0
+  then grind [Int.sign_eq_one_iff_pos]
+  else grind [Int.sign_eq_neg_one_iff_neg]
+
+theorem Int.natAbs_add_of_same_sign (c0 c1 : Int)
+  : c0.sign = c1.sign →
+    (c0 + c1).natAbs = c0.natAbs + c1.natAbs := by
+  intro
+  if _ : c1 = 0 then grind
+  else if _ : c1 > 0
+  then grind [Int.sign_eq_one_iff_pos, Int.natAbs_add_of_nonneg]
+  else have _ : c1 < 0 := by grind
+       grind [Int.sign_eq_neg_one_iff_neg, Int.natAbs_add_of_nonpos]
+
+/- stepIncrementalSlow is a monoid homomorphism
+ from the fixed-signed integers to DialState Nat. -/
+theorem stepIncrementalSlow_hom (c0 c1 : Int)
+  : c0.sign = c1.sign →
+    stepIncrementalSlow (c0 + c1)
+    = ((· + ·) <$> stepIncrementalSlow c0 <*> stepIncrementalSlow c1) := by
+  intros hsign; apply StateT.ext; intro dial0
+  simp [stepIncrementalSlow]
+  rw [Int.natAbs_add_of_same_sign _ _ hsign,
+       ← List.replicate_append_replicate, List.mapM_append,
+       Int.add_same_sign_eq _ _ hsign, hsign]
+  simp
+
+universe u
+def Int.mag_rec :
+  {motive : Int → Sort u} → 
+  (zero : motive 0) → (one : motive 1) → (mone : motive (-1)) →
+  (succ : (n : Int) → 0 ≠ n → motive n → motive n.sign → motive (n + n.sign)) →
+  (t : Int) →
+  motive t := by
+  intros motive h0 h1 hm1 hplus t
+  cases t
+  case ofNat n =>
+    cases n
+    case zero => exact h0
+    case succ n' =>
+      induction n'
+      case zero => exact h1
+      case succ n' ih =>
+        simp ; apply hplus
+        · grind
+        · exact ih
+        · exact h1
+  case negSucc n =>
+    induction n
+    case zero => exact hm1
+    case succ n' ih =>
+      rw [← Int.negSucc_sub_one, Int.sub_eq_add_neg]
+      apply hplus
+      · simp
+      · exact ih
+      · exact hm1
+
+def Int.ring_rec :
+  {motive : Int → Sort u} → 
+  (zero : motive 0) → (one : motive 1) → (mone : motive (-1)) →
+  (add : (n n' : Int) → n ≠ 0 → n.sign = n'.sign → motive n → motive n' → motive (n + n')) →
+  (t : Int) →
+  motive t := by
+  intros motive h0 h1 hm1 hplus t
+  induction t using Int.mag_rec <;> try assumption
+  case succ =>
+    apply hplus <;>
+      (first | assumption | grind [Int.sign_sign])
+
+theorem Int.natAbs_add_sign (n : Int)
+  : n ≠ 0 → (n + n.sign).natAbs = n.natAbs + 1 := by
+  intro h
+  cases n
+  · rw [Int.natAbs_add_of_nonneg]
+    · grind [Int.natAbs_sign_of_ne_zero]
+    · simp
+    · simp
+  · rw [Int.natAbs_add_of_nonpos]
+    · grind [Int.natAbs_sign_of_ne_zero]
+    · grind
+    · simp
+
+theorem stepIncrementalSlow_state (c0 : Int)
+  : stepIncrementalSlow c0 *> pure () = stepDial c0 := by
+  induction c0 using Int.ring_rec
+  case add hn hsign ih0 ih1 =>
+    rw [stepDial_hom, stepIncrementalSlow_hom _ _ hsign, ← ih0, ← ih1]
+    ext : 2 ; simp
+  all_goals
+    ext : 2
+    simp [stepIncrementalSlow, stepAtomic]
+
+@[grind]
+theorem Int.sign_zero (n : Int)
+  : n.sign = 0 ↔ n = 0 := by
+  cases n
+  case ofNat n => cases n <;> simp <;> grind
+  case negSucc n => simp
+
+theorem stepIncremental_zero
+  : stepIncremental 0 = pure 0 := by
+  ext : 2
+  simp [stepIncremental]
+
+theorem stepIncremental_one
+  : stepIncremental 1 = stepAtomic 1 := by
+  ext : 2
+  simp [stepIncremental, stepAtomic, stepDial]
+  split
+  · exfalso ; grind
+  split <;> simp [stepDial0] at * <;> grind
+
+theorem stepIncremental_minus_one
+  : stepIncremental (-1) = stepAtomic (-1) := by
+  ext : 2
+  simp [stepIncremental, stepAtomic, stepDial]
+  split <;> split <;> simp [stepDial0] at *
+  · grind
+  case _ dial h _ =>
+    have heq : dial = (0 : Int) := by grind
+    simp at heq ; grind
+  case _ dial h _ =>
+    have hmodeq : (dialSize : Int) ∣ dial - 1 := by grind
+    have hdial : dial = (1 : Int) := by grind
+    rw [hdial] at h ; simp at h ; subst h
+    contradiction
+  case _ dial _ _ => grind
+
+theorem stepIncremental_succ (c : Int)
+  : 0 < c →
+    stepIncremental (c + 1) =
+    (· + ·) <$> stepIncremental c <*> stepIncremental 1 := by
+  intro h
+  ext : 2
+  rw [stepIncremental_one]
+  simp [stepIncremental, stepDial, stepAtomic, stepDial0]
+  split <;> split <;> simp at * <;> grind
+
+theorem stepIncremental_prec (c : Int)
+  : 0 > c →
+    stepIncremental (c - 1) =
+    (· + ·) <$> stepIncremental c <*> stepIncremental (-1) := by
+  intro h
+  ext : 2
+  rw [stepIncremental_minus_one]
+  simp [stepIncremental, stepDial, stepAtomic, stepDial0]
+  split <;> split <;> split <;> simp at * <;> try grind
+  constructor
+  case _ dial _ _ h =>
+    simp at *
+    generalize hdial0 : (dial + c) % dialSize = dial0 at *
+    have hdial0' : dial0 = 1 := by grind
+    subst hdial0'
+    if h : dial + c <= 0 then grind else
+    if h' : dial + (c - 1) <= 0 then
+      have : dial = 0 := by grind
+      subst dial
+      simp at h
+      omega
+    else
+      have : dial + c = 1 := by grind
+      have : dial + (c - 1) = 0 := by grind
+      grind
+  case _ => grind
+
+theorem eq_stepIncremental_stepIncrementalSlow (c : Int)
+  : stepIncremental c = stepIncrementalSlow c := by
+  induction c using Int.mag_rec
+  · exact stepIncremental_zero
+  · exact stepIncremental_one
+  · exact stepIncremental_minus_one
+  case succ n _ ih _ =>
+    simp [Int.sign]
+    split <;> simp at *
+    · simp [stepIncremental_succ, stepIncrementalSlow_hom] <;> grind
+    · rw [stepIncrementalSlow_hom, ← Int.sub_eq_add_neg, stepIncremental_prec]
+        <;> first | simp | grind
+
+end Day01
